Forgot about EverCrypt.HKDF

providers/evercrypt/fst/EverCrypt.HKDF.fst
@@ -26,17 +26,32 @@ let expand_sha2_512 =
 let extract_sha2_512 =
   mk_extract SHA2_512 EverCrypt.HMAC.compute_sha2_512
 
+let expand_blake2s =
+  mk_expand Blake2S EverCrypt.HMAC.compute_blake2s
 
-let expand a okm prk prklen info infolen len = 
+let extract_blake2s =
+  mk_extract Blake2S EverCrypt.HMAC.compute_blake2s
+
+let expand_blake2b =
+  mk_expand Blake2B EverCrypt.HMAC.compute_blake2b
+
+let extract_blake2b =
+  mk_extract Blake2B EverCrypt.HMAC.compute_blake2b
+
+let expand a okm prk prklen info infolen len =
   match a with
   | SHA1 -> expand_sha1 okm prk prklen info infolen len
   | SHA2_256 -> expand_sha2_256 okm prk prklen info infolen len
   | SHA2_384 -> expand_sha2_384 okm prk prklen info infolen len
   | SHA2_512 -> expand_sha2_512 okm prk prklen info infolen len
+  | Blake2S -> expand_blake2s okm prk prklen info infolen len
+  | Blake2B -> expand_blake2b okm prk prklen info infolen len
 
-let extract a prk salt saltlen ikm ikmlen = 
+let extract a prk salt saltlen ikm ikmlen =
   match a with
   | SHA1 -> extract_sha1 prk salt saltlen ikm ikmlen
   | SHA2_256 -> extract_sha2_256 prk salt saltlen ikm ikmlen
   | SHA2_384 -> extract_sha2_384 prk salt saltlen ikm ikmlen
   | SHA2_512 -> extract_sha2_512 prk salt saltlen ikm ikmlen
+  | Blake2S -> extract_blake2s prk salt saltlen ikm ikmlen
+  | Blake2B -> extract_blake2b prk salt saltlen ikm ikmlen
